WIP fix: A1

nondeterministic_dataflow/table_2/A1.thy
@@ -5,175 +5,296 @@ imports
 begin
 no_notation Sublist.parallel (infixl "\<parallel>" 50)
 
+
+definition "tested n xs ys = map fst (filter (case_prod (=)) (zip (take n xs) (take n ys)))"
+
+lemma tested_diff_Suc:
+  "xs \<noteq> [] \<Longrightarrow> ys \<noteq> [] \<Longrightarrow> hd xs \<noteq> hd ys \<Longrightarrow> tested (Suc n) xs ys = tested n (tl xs) (tl ys)"
+  unfolding tested_def by (simp add: take_Suc)
+
+lemma tested_eq_Suc:
+  "xs \<noteq> [] \<Longrightarrow> ys \<noteq> [] \<Longrightarrow> hd xs = hd ys \<Longrightarrow> tested (Suc n) xs ys = hd xs # tested n (tl xs) (tl ys)"
+  unfolding tested_def by (simp add: take_Suc)
+
+lemma tested_diff_Suc_gen:
+  "length xs > n \<Longrightarrow> length ys > n \<Longrightarrow> xs ! n \<noteq> ys ! n \<Longrightarrow> tested (Suc n) xs ys = tested n xs ys"
+  unfolding tested_def
+  apply (induct n arbitrary: xs ys)
+   apply (auto simp: take_Suc hd_conv_nth)
+  subgoal for n xs ys
+    apply (cases xs; cases ys; simp)
+    done
+  done
+
+lemma tested_eq_Suc_gen:
+  "length xs > n \<Longrightarrow> length ys > n \<Longrightarrow> xs ! n = ys ! n \<Longrightarrow> tested (Suc n) xs ys = tested n xs ys @ [xs ! n]"
+  unfolding tested_def
+  apply (induct n arbitrary: xs ys)
+   apply (auto simp: take_Suc hd_conv_nth)
+  subgoal for n xs ys
+    apply (cases xs; cases ys; simp)
+    done
+  done
+
+lemma length_tested_0[simp]:
+  "tested 0 xs ys = []"
+  unfolding tested_def by simp
+
+
+lemma progress_buffers:
+  assumes "p \<notin> defaults"
+  and "n = min (length (B1' p)) (length (B1 p))"
+  shows "(step Tau)\<^sup>*\<^sup>* (map_op assoc id (map_op projl projr (comp_op Some (case_sum B2'' B2) (id_op B1'' \<parallel> aeq_op (case_sum B1' B1)) (aeq_op (case_sum B3'' B3)))))
+   (map_op assoc id (map_op projl projr (comp_op Some (case_sum (B2''(p := [])) (B2(p := []))) (id_op (B1''(p := [])) \<parallel> aeq_op (case_sum (B1'(p := drop n (B1' p))) (B1(p := drop n (B1 p))))) (aeq_op (case_sum (B3''(p := (B1'' >> B2'' >> B3'') p)) (B3(p := ((B2 >> B3) p) @ tested n (B1' p) (B1 p))))))))"
+  sorry
+
+lemma test_n:
+  assumes "tested n (B3'' p) (B3 p) = []"
+  and "p \<notin> defaults"
+  shows  "(step Tau)\<^sup>*\<^sup>* (map_op assoc id (map_op projl projr (comp_op Some (case_sum B2'' B2) (id_op B1'' \<parallel> aeq_op (case_sum B1' B1)) (aeq_op (case_sum B3'' B3)))))
+    (map_op assoc id (map_op projl projr (comp_op Some (case_sum B2'' B2) (id_op B1'' \<parallel> aeq_op (case_sum B1' B1)) (aeq_op (case_sum (B3''(p := drop n (B3'' p))) (B3(p := drop n (B3 p))))))))"
+  sorry
+
+lemma finds_tested_first_equal:
+  "tested n xs ys = z # zs \<Longrightarrow> n \<le> length xs \<Longrightarrow> n \<le> length ys \<Longrightarrow>
+   \<exists> k. k < n \<and> nth xs k = z \<and> nth ys k = z \<and> tested k xs ys = []"
+  apply (induction n arbitrary: xs ys)
+   apply simp_all
+  subgoal for n xs ys
+    apply (cases xs; cases ys; simp)
+    subgoal for x xs y ys
+      apply hypsubst_thin
+      apply (cases "x = y")
+      apply (metis length_tested_0 list.discI list.sel(1) nat_less_le nth_Cons_0 tested_eq_Suc zero_less_Suc)
+      apply (subst (asm) tested_diff_Suc)
+         apply simp_all
+      apply (drule meta_spec)+
+      apply (drule meta_mp)
+      apply assumption
+      apply (drule meta_mp)
+       apply assumption
+      apply (drule meta_mp)
+       apply assumption
+      apply safe
+      subgoal for k
+        apply (rule exI[of _ "Suc k"])
+        apply (simp add: tested_diff_Suc)
+        done
+      done
+    done
+  done
+
+lemma tested_all:
+  "tested (min (length A) (length C)) A C = map fst (filter (case_prod (=)) (zip A C))"
+  unfolding tested_def by (metis map_fst_zip_take map_snd_zip_take zip_map_fst_snd)
+
+
+lemma tested_min_helper:
+  " B1' = drop m C \<Longrightarrow>
+    B1 = drop m A \<Longrightarrow>
+    B3 @ B2 = tested m A C \<Longrightarrow>
+    tested (min (length A) (length C)) A C = B3 @ B2 @ tested (min (length B1) (length B1')) B1 B1'"
+  apply (simp (no_asm) add: tested_all)
+  apply (auto 0 0 simp add: tested_def)
+  apply (metis append.assoc append_take_drop_id drop_zip filter_append map_append take_zip)
+  done
+
+lemma tested_comm:
+  "tested n xs ys = tested n ys xs"
+  apply (induct n arbitrary: xs ys)
+   apply simp_all
+  subgoal for n xs ys
+    apply (cases xs; cases ys; simp)
+    apply (simp_all add: tested_def)
+    done
+  done  
+
+  
 section \<open>Axiom A1: Equality test commutes with identity\<close>
 lemma A1_gen:
-  \<open>map_op projl projr (comp_op Some (case_sum buf2 buf2') (aeq_op (case_sum buf1 buf1') \<parallel> id_op buf1'') (aeq_op (case_sum buf3 buf3')))
-  ~ map_op (case_sum Inr Inl) id (map_op projl projr (comp_op Some (case_sum buf2' buf2) (id_op buf1'' \<parallel> aeq_op (case_sum buf1 buf1')) (aeq_op (case_sum buf3' buf3))))\<close>
-proof (coinduction arbitrary: buf1 buf1' buf1'' buf2 buf2' buf3 buf3' rule: bisim_coinduct_upto)
-  case BISIM
+  assumes "A = A1 >> A2 >> A3"
+  and "B'' = B1'' >> B2'' >> B3''"
+  and "\<forall> p. \<exists> m n C'. A1'' p = drop n (B'' p) \<and> A1' p = drop n (C' p) \<and> B1' p = drop m (C' p) \<and> B1 p = drop m (A p) \<and>
+       (A2' >> A3') p = tested n (C' p) (B'' p) \<and> (B2 >> B3) p = tested m (A p) (C' p) \<and>
+        n \<le> length (C' p) \<and> n \<le> length (B'' p) \<and> m \<le> length (C' p) \<and> m \<le> length (A p)"
+shows  \<open>map_op projl projr (comp_op Some (case_sum A2' A2) (aeq_op (case_sum A1'' A1') \<parallel> id_op A1) (aeq_op (case_sum A3' A3)))
+  \<approx> map_op assoc id (map_op projl projr (comp_op Some (case_sum B2'' B2) (id_op B1'' \<parallel> aeq_op (case_sum B1' B1)) (aeq_op (case_sum B3'' B3))))\<close>
+  unfolding pcomp_op_def
+using assms proof (coinduction arbitrary:A A1 A1' B1' A2 A3 A1'' A2' A3' B1 B2 B3 B'' B1'' B2'' B3'' rule: wbisim_coinduct)
+  case SIM1
   then show ?case
-    unfolding sim_def pcomp_op_def
-  proof (intro allI conjI impI)
-    fix io :: "(('a + 'a) + 'a, 'a, 'b) IO"
-      and op1' :: "(('a + 'a) + 'a, 'a, 'b) op"
-    assume H: "step io (map_op projl projr (comp_op Some (case_sum buf2 buf2') (comp_op (\<lambda>_. None) (\<lambda>_. []) (aeq_op (case_sum buf1 buf1')) (id_op buf1'')) (aeq_op (case_sum buf3 buf3')))) op1'"
-    show "\<exists>op2'. step io (map_op (case_sum Inr Inl) id (map_op projl projr (comp_op Some (case_sum buf2' buf2) (comp_op (\<lambda>_. None) (\<lambda>_. []) (id_op buf1'') (aeq_op (case_sum buf1 buf1'))) (aeq_op (case_sum buf3' buf3))))) op2' \<and> bisim_cong (\<lambda>s t. \<exists>buf1 buf1' buf1'' buf2 buf2' buf3 buf3'. s = map_op projl projr (comp_op Some (case_sum buf2 buf2') (comp_op (\<lambda>_. None) (\<lambda>_. []) (aeq_op (case_sum buf1 buf1')) (id_op buf1'')) (aeq_op (case_sum buf3 buf3'))) \<and> t = map_op (case_sum Inr Inl) id (map_op projl projr (comp_op Some (case_sum buf2' buf2) (comp_op (\<lambda>_. None) (\<lambda>_. []) (id_op buf1'') (aeq_op (case_sum buf1 buf1'))) (aeq_op (case_sum buf3' buf3))))) op1' op2'"
-    proof -
-      have "\<exists>op2'. step (Inp (Inl (Inl pb)) y) (map_op (case_sum Inr Inl) id (map_op projl projr (comp_op Some (case_sum buf2' buf2) (comp_op (\<lambda>_. None) (\<lambda>_. []) (id_op buf1'') (aeq_op (case_sum buf1 buf1'))) (aeq_op (case_sum buf3' buf3))))) op2' \<and> bisim_cong (\<lambda>s t. \<exists>buf1 buf1' buf1'' buf2 buf2' buf3 buf3'. s = map_op projl projr (comp_op Some (case_sum buf2 buf2') (comp_op (\<lambda>_. None) (\<lambda>_. []) (aeq_op (case_sum buf1 buf1')) (id_op buf1'')) (aeq_op (case_sum buf3 buf3'))) \<and> t = map_op (case_sum Inr Inl) id (map_op projl projr (comp_op Some (case_sum buf2' buf2) (comp_op (\<lambda>_. None) (\<lambda>_. []) (id_op buf1'') (aeq_op (case_sum buf1 buf1'))) (aeq_op (case_sum buf3' buf3))))) (map_op projl projr (comp_op Some (case_sum buf2 buf2') (comp_op (\<lambda>_. None) (\<lambda>_. []) (aeq_op (case_sum (BENQ pb y buf1) buf1')) (id_op buf1'')) (aeq_op (case_sum buf3 buf3')))) op2'"
-        if "pb \<notin> defaults"
-        for pb :: 'a
-          and y :: 'b
-        using that by (fastforce intro: bc_base)
-      moreover have "\<exists>op2'. step (Inp (Inl (Inr pb)) y) (map_op (case_sum Inr Inl) id (map_op projl projr (comp_op Some (case_sum buf2' buf2) (comp_op (\<lambda>_. None) (\<lambda>_. []) (id_op buf1'') (aeq_op (case_sum buf1 buf1'))) (aeq_op (case_sum buf3' buf3))))) op2' \<and> bisim_cong (\<lambda>s t. \<exists>buf1 buf1' buf1'' buf2 buf2' buf3 buf3'. s = map_op projl projr (comp_op Some (case_sum buf2 buf2') (comp_op (\<lambda>_. None) (\<lambda>_. []) (aeq_op (case_sum buf1 buf1')) (id_op buf1'')) (aeq_op (case_sum buf3 buf3'))) \<and> t = map_op (case_sum Inr Inl) id (map_op projl projr (comp_op Some (case_sum buf2' buf2) (comp_op (\<lambda>_. None) (\<lambda>_. []) (id_op buf1'') (aeq_op (case_sum buf1 buf1'))) (aeq_op (case_sum buf3' buf3))))) (map_op projl projr (comp_op Some (case_sum buf2 buf2') (comp_op (\<lambda>_. None) (\<lambda>_. []) (aeq_op (case_sum buf1 (BENQ pb y buf1'))) (id_op buf1'')) (aeq_op (case_sum buf3 buf3')))) op2'"
-        if "pb \<notin> defaults"
-        for pb :: 'a
-          and y :: 'b
-        using that by (fastforce intro: bc_base)
-      moreover have "\<exists>op2'. step (Inp (Inr pb) xb) (map_op (case_sum Inr Inl) id (map_op projl projr (comp_op Some (case_sum buf2' buf2) (comp_op (\<lambda>_. None) (\<lambda>_. []) (id_op buf1'') (aeq_op (case_sum buf1 buf1'))) (aeq_op (case_sum buf3' buf3))))) op2' \<and> bisim_cong (\<lambda>s t. \<exists>buf1 buf1' buf1'' buf2 buf2' buf3 buf3'. s = map_op projl projr (comp_op Some (case_sum buf2 buf2') (comp_op (\<lambda>_. None) (\<lambda>_. []) (aeq_op (case_sum buf1 buf1')) (id_op buf1'')) (aeq_op (case_sum buf3 buf3'))) \<and> t = map_op (case_sum Inr Inl) id (map_op projl projr (comp_op Some (case_sum buf2' buf2) (comp_op (\<lambda>_. None) (\<lambda>_. []) (id_op buf1'') (aeq_op (case_sum buf1 buf1'))) (aeq_op (case_sum buf3' buf3))))) (map_op projl projr (comp_op Some (case_sum buf2 buf2') (comp_op (\<lambda>_. None) (\<lambda>_. []) (aeq_op (case_sum buf1 buf1')) (id_op (BENQ pb xb buf1''))) (aeq_op (case_sum buf3 buf3')))) op2'"
-        if "pb \<notin> defaults"
-        for pb :: 'a
-          and xb :: 'b
-        using that by (fastforce intro: bc_base)
-      moreover have "\<exists>op2'. step (Out pa (BHD pa buf3')) (map_op (case_sum Inr Inl) id (map_op projl projr (comp_op Some (case_sum buf2' buf2) (comp_op (\<lambda>_. None) (\<lambda>_. []) (id_op buf1'') (aeq_op (case_sum buf1 buf1'))) (aeq_op (case_sum buf3' buf3))))) op2' \<and> bisim_cong (\<lambda>s t. \<exists>buf1 buf1' buf1'' buf2 buf2' buf3 buf3'. s = map_op projl projr (comp_op Some (case_sum buf2 buf2') (comp_op (\<lambda>_. None) (\<lambda>_. []) (aeq_op (case_sum buf1 buf1')) (id_op buf1'')) (aeq_op (case_sum buf3 buf3'))) \<and> t = map_op (case_sum Inr Inl) id (map_op projl projr (comp_op Some (case_sum buf2' buf2) (comp_op (\<lambda>_. None) (\<lambda>_. []) (id_op buf1'') (aeq_op (case_sum buf1 buf1'))) (aeq_op (case_sum buf3' buf3))))) (map_op projl projr (comp_op Some (case_sum buf2 buf2') (comp_op (\<lambda>_. None) (\<lambda>_. []) (aeq_op (case_sum buf1 buf1')) (id_op buf1'')) (aeq_op (case_sum (BTL pa buf3) (BTL pa buf3'))))) op2'"
-        if "buf3 pa \<noteq> []"
-          and "buf3' pa \<noteq> []"
-          and "BHD pa buf3 = BHD pa buf3'"
-          and "pa \<notin> defaults"
-        for pa :: 'a
-        using that by (fastforce intro: bc_base)
-      moreover have "\<exists>op2'. step Tau (map_op (case_sum Inr Inl) id (map_op projl projr (comp_op Some (case_sum buf2' buf2) (comp_op (\<lambda>_. None) (\<lambda>_. []) (id_op buf1'') (aeq_op (case_sum buf1 buf1'))) (aeq_op (case_sum buf3' buf3))))) op2' \<and> bisim_cong (\<lambda>s t. \<exists>buf1 buf1' buf1'' buf2 buf2' buf3 buf3'. s = map_op projl projr (comp_op Some (case_sum buf2 buf2') (comp_op (\<lambda>_. None) (\<lambda>_. []) (aeq_op (case_sum buf1 buf1')) (id_op buf1'')) (aeq_op (case_sum buf3 buf3'))) \<and> t = map_op (case_sum Inr Inl) id (map_op projl projr (comp_op Some (case_sum buf2' buf2) (comp_op (\<lambda>_. None) (\<lambda>_. []) (id_op buf1'') (aeq_op (case_sum buf1 buf1'))) (aeq_op (case_sum buf3' buf3))))) (map_op projl projr (comp_op Some (case_sum buf2 (BENQ pb (BHD pb buf1'') buf2')) (comp_op (\<lambda>_. None) (\<lambda>_. []) (aeq_op (case_sum buf1 buf1')) (id_op (BTL pb buf1''))) (aeq_op (case_sum buf3 buf3')))) op2'"
-        if "pb \<notin> defaults"
-          and "buf1'' pb \<noteq> []"
-        for pb :: 'a
-        using that by (fastforce intro: bc_base)
-      moreover have "\<exists>op2'. step Tau (map_op (case_sum Inr Inl) id (map_op projl projr (comp_op Some (case_sum buf2' buf2) (comp_op (\<lambda>_. None) (\<lambda>_. []) (id_op buf1'') (aeq_op (case_sum buf1 buf1'))) (aeq_op (case_sum buf3' buf3))))) op2' \<and> bisim_cong (\<lambda>s t. \<exists>buf1 buf1' buf1'' buf2 buf2' buf3 buf3'. s = map_op projl projr (comp_op Some (case_sum buf2 buf2') (comp_op (\<lambda>_. None) (\<lambda>_. []) (aeq_op (case_sum buf1 buf1')) (id_op buf1'')) (aeq_op (case_sum buf3 buf3'))) \<and> t = map_op (case_sum Inr Inl) id (map_op projl projr (comp_op Some (case_sum buf2' buf2) (comp_op (\<lambda>_. None) (\<lambda>_. []) (id_op buf1'') (aeq_op (case_sum buf1 buf1'))) (aeq_op (case_sum buf3' buf3))))) (map_op projl projr (comp_op Some (case_sum (BENQ pb (BHD pb buf1') buf2) buf2') (comp_op (\<lambda>_. None) (\<lambda>_. []) (aeq_op (case_sum (BTL pb buf1) (BTL pb buf1'))) (id_op buf1'')) (aeq_op (case_sum buf3 buf3')))) op2'"
-        if "buf1 pb \<noteq> []"
-          and "buf1' pb \<noteq> []"
-          and "BHD pb buf1 = BHD pb buf1'"
-          and "pb \<notin> defaults"
-        for pb :: 'a
-        using that by (fastforce intro: bc_base)
-      moreover have "\<exists>op2'. step Tau (map_op (case_sum Inr Inl) id (map_op projl projr (comp_op Some (case_sum buf2' buf2) (comp_op (\<lambda>_. None) (\<lambda>_. []) (id_op buf1'') (aeq_op (case_sum buf1 buf1'))) (aeq_op (case_sum buf3' buf3))))) op2' \<and> bisim_cong (\<lambda>s t. \<exists>buf1 buf1' buf1'' buf2 buf2' buf3 buf3'. s = map_op projl projr (comp_op Some (case_sum buf2 buf2') (comp_op (\<lambda>_. None) (\<lambda>_. []) (aeq_op (case_sum buf1 buf1')) (id_op buf1'')) (aeq_op (case_sum buf3 buf3'))) \<and> t = map_op (case_sum Inr Inl) id (map_op projl projr (comp_op Some (case_sum buf2' buf2) (comp_op (\<lambda>_. None) (\<lambda>_. []) (id_op buf1'') (aeq_op (case_sum buf1 buf1'))) (aeq_op (case_sum buf3' buf3))))) (map_op projl projr (comp_op Some (case_sum (BTL pa buf2) buf2') (comp_op (\<lambda>_. None) (\<lambda>_. []) (aeq_op (case_sum buf1 buf1')) (id_op buf1'')) (aeq_op (case_sum (BENQ pa (BHD pa buf2) buf3) buf3')))) op2'"
-        if "buf2 pa \<noteq> []"
-          and "pa \<notin> defaults"
-        for pa :: 'a
-        using that by (fastforce intro: bc_base)
-      moreover have "\<exists>op2'. step Tau (map_op (case_sum Inr Inl) id (map_op projl projr (comp_op Some (case_sum buf2' buf2) (comp_op (\<lambda>_. None) (\<lambda>_. []) (id_op buf1'') (aeq_op (case_sum buf1 buf1'))) (aeq_op (case_sum buf3' buf3))))) op2' \<and> bisim_cong (\<lambda>s t. \<exists>buf1 buf1' buf1'' buf2 buf2' buf3 buf3'. s = map_op projl projr (comp_op Some (case_sum buf2 buf2') (comp_op (\<lambda>_. None) (\<lambda>_. []) (aeq_op (case_sum buf1 buf1')) (id_op buf1'')) (aeq_op (case_sum buf3 buf3'))) \<and> t = map_op (case_sum Inr Inl) id (map_op projl projr (comp_op Some (case_sum buf2' buf2) (comp_op (\<lambda>_. None) (\<lambda>_. []) (id_op buf1'') (aeq_op (case_sum buf1 buf1'))) (aeq_op (case_sum buf3' buf3))))) (map_op projl projr (comp_op Some (case_sum buf2 (BTL pa buf2')) (comp_op (\<lambda>_. None) (\<lambda>_. []) (aeq_op (case_sum buf1 buf1')) (id_op buf1'')) (aeq_op (case_sum buf3 (BENQ pa (BHD pa buf2') buf3'))))) op2'"
-        if "buf2' pa \<noteq> []"
-          and "pa \<notin> defaults"
-        for pa :: 'a
-        using that by (fastforce intro: bc_base)
-      moreover have "\<exists>op2'. step Tau (map_op (case_sum Inr Inl) id (map_op projl projr (comp_op Some (case_sum buf2' buf2) (comp_op (\<lambda>_. None) (\<lambda>_. []) (id_op buf1'') (aeq_op (case_sum buf1 buf1'))) (aeq_op (case_sum buf3' buf3))))) op2' \<and> bisim_cong (\<lambda>s t. \<exists>buf1 buf1' buf1'' buf2 buf2' buf3 buf3'. s = map_op projl projr (comp_op Some (case_sum buf2 buf2') (comp_op (\<lambda>_. None) (\<lambda>_. []) (aeq_op (case_sum buf1 buf1')) (id_op buf1'')) (aeq_op (case_sum buf3 buf3'))) \<and> t = map_op (case_sum Inr Inl) id (map_op projl projr (comp_op Some (case_sum buf2' buf2) (comp_op (\<lambda>_. None) (\<lambda>_. []) (id_op buf1'') (aeq_op (case_sum buf1 buf1'))) (aeq_op (case_sum buf3' buf3))))) (map_op projl projr (comp_op Some (case_sum buf2 buf2') (comp_op (\<lambda>_. None) (\<lambda>_. []) (aeq_op (case_sum (BTL pb buf1) (BTL pb buf1'))) (id_op buf1'')) (aeq_op (case_sum buf3 buf3')))) op2'"
-        if "buf1 pb \<noteq> []"
-          and "buf1' pb \<noteq> []"
-          and "BHD pb buf1 \<noteq> BHD pb buf1'"
-          and "pb \<notin> defaults"
-        for pb :: 'a
-      proof -
-        have \<open>step Tau
-       (comp_op Some (case_sum buf2' buf2)
-         (comp_op (\<lambda>_. None) (\<lambda>_. []) (id_op buf1'') (aeq_op (case_sum buf1 buf1')))
-         (aeq_op (case_sum buf3' buf3)))
-       (comp_op Some (case_sum buf2' buf2)
-         (comp_op (\<lambda>_. None) (\<lambda>_. []) (id_op buf1'')
-           (aeq_op (case_sum (BTL pb buf1) (BTL pb buf1'))))
-         (aeq_op (case_sum buf3' buf3))) \<close>
-          using that by fastforce
-        thus ?thesis by (fastforce intro: bc_base)
-      qed
-      moreover have "\<exists>op2'. step Tau (map_op (case_sum Inr Inl) id (map_op projl projr (comp_op Some (case_sum buf2' buf2) (comp_op (\<lambda>_. None) (\<lambda>_. []) (id_op buf1'') (aeq_op (case_sum buf1 buf1'))) (aeq_op (case_sum buf3' buf3))))) op2' \<and> bisim_cong (\<lambda>s t. \<exists>buf1 buf1' buf1'' buf2 buf2' buf3 buf3'. s = map_op projl projr (comp_op Some (case_sum buf2 buf2') (comp_op (\<lambda>_. None) (\<lambda>_. []) (aeq_op (case_sum buf1 buf1')) (id_op buf1'')) (aeq_op (case_sum buf3 buf3'))) \<and> t = map_op (case_sum Inr Inl) id (map_op projl projr (comp_op Some (case_sum buf2' buf2) (comp_op (\<lambda>_. None) (\<lambda>_. []) (id_op buf1'') (aeq_op (case_sum buf1 buf1'))) (aeq_op (case_sum buf3' buf3))))) (map_op projl projr (comp_op Some (case_sum buf2 buf2') (comp_op (\<lambda>_. None) (\<lambda>_. []) (aeq_op (case_sum buf1 buf1')) (id_op buf1'')) (aeq_op (case_sum (BTL pa buf3) (BTL pa buf3'))))) op2'"
-        if "buf3 pa \<noteq> []"
-          and "buf3' pa \<noteq> []"
-          and "BHD pa buf3 \<noteq> BHD pa buf3'"
-          and "pa \<notin> defaults"
-        for pa :: 'a
-        using that by (intro exI conjI[rotated, OF bc_base], auto)
-      ultimately show ?thesis
-        using H by (auto elim !: step_map_op_elim step_comp_op_elim step_aeq_op_elim step_id_op_cases)
-    qed
-  next
-    fix io :: "(('a + 'a) + 'a, 'a, 'b) IO"
-      and op1' :: "(('a + 'a) + 'a, 'a, 'b) op"
-    assume H: "step io (map_op (case_sum Inr Inl) id (map_op projl projr (comp_op Some (case_sum buf2' buf2) (comp_op (\<lambda>_. None) (\<lambda>_. []) (id_op buf1'') (aeq_op (case_sum buf1 buf1'))) (aeq_op (case_sum buf3' buf3))))) op1'"
-    show "\<exists>op2'. step io (map_op projl projr (comp_op Some (case_sum buf2 buf2') (comp_op (\<lambda>_. None) (\<lambda>_. []) (aeq_op (case_sum buf1 buf1')) (id_op buf1'')) (aeq_op (case_sum buf3 buf3')))) op2' \<and> bisim_cong (\<lambda>s t. \<exists>buf1 buf1' buf1'' buf2 buf2' buf3 buf3'. s = map_op projl projr (comp_op Some (case_sum buf2 buf2') (comp_op (\<lambda>_. None) (\<lambda>_. []) (aeq_op (case_sum buf1 buf1')) (id_op buf1'')) (aeq_op (case_sum buf3 buf3'))) \<and> t = map_op (case_sum Inr Inl) id (map_op projl projr (comp_op Some (case_sum buf2' buf2) (comp_op (\<lambda>_. None) (\<lambda>_. []) (id_op buf1'') (aeq_op (case_sum buf1 buf1'))) (aeq_op (case_sum buf3' buf3))))) op1' op2'"
-    proof -
-      have "\<exists>op2'. step (Inp (Inr pb) xb) (map_op projl projr (comp_op Some (case_sum buf2 buf2') (comp_op (\<lambda>_. None) (\<lambda>_. []) (aeq_op (case_sum buf1 buf1')) (id_op buf1'')) (aeq_op (case_sum buf3 buf3')))) op2' \<and> bisim_cong (\<lambda>s t. \<exists>buf1 buf1' buf1'' buf2 buf2' buf3 buf3'. s = map_op projl projr (comp_op Some (case_sum buf2 buf2') (comp_op (\<lambda>_. None) (\<lambda>_. []) (aeq_op (case_sum buf1 buf1')) (id_op buf1'')) (aeq_op (case_sum buf3 buf3'))) \<and> t = map_op (case_sum Inr Inl) id (map_op projl projr (comp_op Some (case_sum buf2' buf2) (comp_op (\<lambda>_. None) (\<lambda>_. []) (id_op buf1'') (aeq_op (case_sum buf1 buf1'))) (aeq_op (case_sum buf3' buf3))))) (map_op (case_sum Inr Inl) id (map_op projl projr (comp_op Some (case_sum buf2' buf2) (comp_op (\<lambda>_. None) (\<lambda>_. []) (id_op (BENQ pb xb buf1'')) (aeq_op (case_sum buf1 buf1'))) (aeq_op (case_sum buf3' buf3))))) op2'"
-        if "pb \<notin> defaults"
-        for pb :: 'a
-          and xb :: 'b
-        using that by (fastforce intro: bc_sym[OF bc_base])
-      moreover have "\<exists>op2'. step (Inp (Inl (Inl pb)) y) (map_op projl projr (comp_op Some (case_sum buf2 buf2') (comp_op (\<lambda>_. None) (\<lambda>_. []) (aeq_op (case_sum buf1 buf1')) (id_op buf1'')) (aeq_op (case_sum buf3 buf3')))) op2' \<and> bisim_cong (\<lambda>s t. \<exists>buf1 buf1' buf1'' buf2 buf2' buf3 buf3'. s = map_op projl projr (comp_op Some (case_sum buf2 buf2') (comp_op (\<lambda>_. None) (\<lambda>_. []) (aeq_op (case_sum buf1 buf1')) (id_op buf1'')) (aeq_op (case_sum buf3 buf3'))) \<and> t = map_op (case_sum Inr Inl) id (map_op projl projr (comp_op Some (case_sum buf2' buf2) (comp_op (\<lambda>_. None) (\<lambda>_. []) (id_op buf1'') (aeq_op (case_sum buf1 buf1'))) (aeq_op (case_sum buf3' buf3))))) (map_op (case_sum Inr Inl) id (map_op projl projr (comp_op Some (case_sum buf2' buf2) (comp_op (\<lambda>_. None) (\<lambda>_. []) (id_op buf1'') (aeq_op (case_sum (BENQ pb y buf1) buf1'))) (aeq_op (case_sum buf3' buf3))))) op2'"
-        if "pb \<notin> defaults"
-        for pb :: 'a
-          and y :: 'b
-        using that by (fastforce intro: bc_sym[OF bc_base])
-      moreover have "\<exists>op2'. step (Inp (Inl (Inr pb)) y) (map_op projl projr (comp_op Some (case_sum buf2 buf2') (comp_op (\<lambda>_. None) (\<lambda>_. []) (aeq_op (case_sum buf1 buf1')) (id_op buf1'')) (aeq_op (case_sum buf3 buf3')))) op2' \<and> bisim_cong (\<lambda>s t. \<exists>buf1 buf1' buf1'' buf2 buf2' buf3 buf3'. s = map_op projl projr (comp_op Some (case_sum buf2 buf2') (comp_op (\<lambda>_. None) (\<lambda>_. []) (aeq_op (case_sum buf1 buf1')) (id_op buf1'')) (aeq_op (case_sum buf3 buf3'))) \<and> t = map_op (case_sum Inr Inl) id (map_op projl projr (comp_op Some (case_sum buf2' buf2) (comp_op (\<lambda>_. None) (\<lambda>_. []) (id_op buf1'') (aeq_op (case_sum buf1 buf1'))) (aeq_op (case_sum buf3' buf3))))) (map_op (case_sum Inr Inl) id (map_op projl projr (comp_op Some (case_sum buf2' buf2) (comp_op (\<lambda>_. None) (\<lambda>_. []) (id_op buf1'') (aeq_op (case_sum buf1 (BENQ pb y buf1')))) (aeq_op (case_sum buf3' buf3))))) op2'"
-        if "pb \<notin> defaults"
-        for pb :: 'a
-          and y :: 'b
-        using that by (fastforce intro: bc_sym[OF bc_base])
-      moreover have "\<exists>op2'. step (Out pa (BHD pa buf3)) (map_op projl projr (comp_op Some (case_sum buf2 buf2') (comp_op (\<lambda>_. None) (\<lambda>_. []) (aeq_op (case_sum buf1 buf1')) (id_op buf1'')) (aeq_op (case_sum buf3 buf3')))) op2' \<and> bisim_cong (\<lambda>s t. \<exists>buf1 buf1' buf1'' buf2 buf2' buf3 buf3'. s = map_op projl projr (comp_op Some (case_sum buf2 buf2') (comp_op (\<lambda>_. None) (\<lambda>_. []) (aeq_op (case_sum buf1 buf1')) (id_op buf1'')) (aeq_op (case_sum buf3 buf3'))) \<and> t = map_op (case_sum Inr Inl) id (map_op projl projr (comp_op Some (case_sum buf2' buf2) (comp_op (\<lambda>_. None) (\<lambda>_. []) (id_op buf1'') (aeq_op (case_sum buf1 buf1'))) (aeq_op (case_sum buf3' buf3))))) (map_op (case_sum Inr Inl) id (map_op projl projr (comp_op Some (case_sum buf2' buf2) (comp_op (\<lambda>_. None) (\<lambda>_. []) (id_op buf1'') (aeq_op (case_sum buf1 buf1'))) (aeq_op (case_sum (BTL pa buf3') (BTL pa buf3)))))) op2'"
-        if "buf3' pa \<noteq> []"
-          and "buf3 pa \<noteq> []"
-          and "BHD pa buf3' = BHD pa buf3"
-          and "pa \<notin> defaults"
-        for pa :: 'a
-        using that by (fastforce intro: bc_sym[OF bc_base])
-      moreover have "\<exists>op2'. step Tau (map_op projl projr (comp_op Some (case_sum buf2 buf2') (comp_op (\<lambda>_. None) (\<lambda>_. []) (aeq_op (case_sum buf1 buf1')) (id_op buf1'')) (aeq_op (case_sum buf3 buf3')))) op2' \<and> bisim_cong (\<lambda>s t. \<exists>buf1 buf1' buf1'' buf2 buf2' buf3 buf3'. s = map_op projl projr (comp_op Some (case_sum buf2 buf2') (comp_op (\<lambda>_. None) (\<lambda>_. []) (aeq_op (case_sum buf1 buf1')) (id_op buf1'')) (aeq_op (case_sum buf3 buf3'))) \<and> t = map_op (case_sum Inr Inl) id (map_op projl projr (comp_op Some (case_sum buf2' buf2) (comp_op (\<lambda>_. None) (\<lambda>_. []) (id_op buf1'') (aeq_op (case_sum buf1 buf1'))) (aeq_op (case_sum buf3' buf3))))) (map_op (case_sum Inr Inl) id (map_op projl projr (comp_op Some (case_sum buf2' (BENQ pb (BHD pb buf1') buf2)) (comp_op (\<lambda>_. None) (\<lambda>_. []) (id_op buf1'') (aeq_op (case_sum (BTL pb buf1) (BTL pb buf1')))) (aeq_op (case_sum buf3' buf3))))) op2'"
-        if "buf1 pb \<noteq> []"
-          and "buf1' pb \<noteq> []"
-          and "BHD pb buf1 = BHD pb buf1'"
-          and "pb \<notin> defaults"
-        for pb :: 'a
-        using that by (fastforce intro: bc_sym[OF bc_base])
-      moreover have "\<exists>op2'. step Tau (map_op projl projr (comp_op Some (case_sum buf2 buf2') (comp_op (\<lambda>_. None) (\<lambda>_. []) (aeq_op (case_sum buf1 buf1')) (id_op buf1'')) (aeq_op (case_sum buf3 buf3')))) op2' \<and> bisim_cong (\<lambda>s t. \<exists>buf1 buf1' buf1'' buf2 buf2' buf3 buf3'. s = map_op projl projr (comp_op Some (case_sum buf2 buf2') (comp_op (\<lambda>_. None) (\<lambda>_. []) (aeq_op (case_sum buf1 buf1')) (id_op buf1'')) (aeq_op (case_sum buf3 buf3'))) \<and> t = map_op (case_sum Inr Inl) id (map_op projl projr (comp_op Some (case_sum buf2' buf2) (comp_op (\<lambda>_. None) (\<lambda>_. []) (id_op buf1'') (aeq_op (case_sum buf1 buf1'))) (aeq_op (case_sum buf3' buf3))))) (map_op (case_sum Inr Inl) id (map_op projl projr (comp_op Some (case_sum (BENQ pb (BHD pb buf1'') buf2') buf2) (comp_op (\<lambda>_. None) (\<lambda>_. []) (id_op (BTL pb buf1'')) (aeq_op (case_sum buf1 buf1'))) (aeq_op (case_sum buf3' buf3))))) op2'"
-        if "pb \<notin> defaults"
-          and "buf1'' pb \<noteq> []"
-        for pb :: 'a
-        using that by (fastforce intro: bc_sym[OF bc_base])
-      moreover have "\<exists>op2'. step Tau (map_op projl projr (comp_op Some (case_sum buf2 buf2') (comp_op (\<lambda>_. None) (\<lambda>_. []) (aeq_op (case_sum buf1 buf1')) (id_op buf1'')) (aeq_op (case_sum buf3 buf3')))) op2' \<and> bisim_cong (\<lambda>s t. \<exists>buf1 buf1' buf1'' buf2 buf2' buf3 buf3'. s = map_op projl projr (comp_op Some (case_sum buf2 buf2') (comp_op (\<lambda>_. None) (\<lambda>_. []) (aeq_op (case_sum buf1 buf1')) (id_op buf1'')) (aeq_op (case_sum buf3 buf3'))) \<and> t = map_op (case_sum Inr Inl) id (map_op projl projr (comp_op Some (case_sum buf2' buf2) (comp_op (\<lambda>_. None) (\<lambda>_. []) (id_op buf1'') (aeq_op (case_sum buf1 buf1'))) (aeq_op (case_sum buf3' buf3))))) (map_op (case_sum Inr Inl) id (map_op projl projr (comp_op Some (case_sum (BTL pa buf2') buf2) (comp_op (\<lambda>_. None) (\<lambda>_. []) (id_op buf1'') (aeq_op (case_sum buf1 buf1'))) (aeq_op (case_sum (BENQ pa (BHD pa buf2') buf3') buf3))))) op2'"
-        if "buf2' pa \<noteq> []"
-          and "pa \<notin> defaults"
-        for pa :: 'a
-        using that by (fastforce intro: bc_sym[OF bc_base])
-      moreover have "\<exists>op2'. step Tau (map_op projl projr (comp_op Some (case_sum buf2 buf2') (comp_op (\<lambda>_. None) (\<lambda>_. []) (aeq_op (case_sum buf1 buf1')) (id_op buf1'')) (aeq_op (case_sum buf3 buf3')))) op2' \<and> bisim_cong (\<lambda>s t. \<exists>buf1 buf1' buf1'' buf2 buf2' buf3 buf3'. s = map_op projl projr (comp_op Some (case_sum buf2 buf2') (comp_op (\<lambda>_. None) (\<lambda>_. []) (aeq_op (case_sum buf1 buf1')) (id_op buf1'')) (aeq_op (case_sum buf3 buf3'))) \<and> t = map_op (case_sum Inr Inl) id (map_op projl projr (comp_op Some (case_sum buf2' buf2) (comp_op (\<lambda>_. None) (\<lambda>_. []) (id_op buf1'') (aeq_op (case_sum buf1 buf1'))) (aeq_op (case_sum buf3' buf3))))) (map_op (case_sum Inr Inl) id (map_op projl projr (comp_op Some (case_sum buf2' (BTL pa buf2)) (comp_op (\<lambda>_. None) (\<lambda>_. []) (id_op buf1'') (aeq_op (case_sum buf1 buf1'))) (aeq_op (case_sum buf3' (BENQ pa (BHD pa buf2) buf3)))))) op2'"
-        if "buf2 pa \<noteq> []"
-          and "pa \<notin> defaults"
-        for pa :: 'a
-        using that by (fastforce intro: bc_sym[OF bc_base])
-      moreover have "\<exists>op2'. step Tau (map_op projl projr (comp_op Some (case_sum buf2 buf2') (comp_op (\<lambda>_. None) (\<lambda>_. []) (aeq_op (case_sum buf1 buf1')) (id_op buf1'')) (aeq_op (case_sum buf3 buf3')))) op2' \<and> bisim_cong (\<lambda>s t. \<exists>buf1 buf1' buf1'' buf2 buf2' buf3 buf3'. s = map_op projl projr (comp_op Some (case_sum buf2 buf2') (comp_op (\<lambda>_. None) (\<lambda>_. []) (aeq_op (case_sum buf1 buf1')) (id_op buf1'')) (aeq_op (case_sum buf3 buf3'))) \<and> t = map_op (case_sum Inr Inl) id (map_op projl projr (comp_op Some (case_sum buf2' buf2) (comp_op (\<lambda>_. None) (\<lambda>_. []) (id_op buf1'') (aeq_op (case_sum buf1 buf1'))) (aeq_op (case_sum buf3' buf3))))) (map_op (case_sum Inr Inl) id (map_op projl projr (comp_op Some (case_sum buf2' buf2) (comp_op (\<lambda>_. None) (\<lambda>_. []) (id_op buf1'') (aeq_op (case_sum (BTL pb buf1) (BTL pb buf1')))) (aeq_op (case_sum buf3' buf3))))) op2'"
-        if "buf1 pb \<noteq> []"
-          and "buf1' pb \<noteq> []"
-          and "BHD pb buf1 \<noteq> BHD pb buf1'"
-          and "pb \<notin> defaults"
-        for pb :: 'a
-      proof -
-        have \<open>step Tau
-     (comp_op Some (case_sum buf2 buf2')
-       (comp_op (\<lambda>_. None) (\<lambda>_. []) (aeq_op (case_sum buf1 buf1')) (id_op buf1''))
-       (aeq_op (case_sum buf3 buf3')))
-     (comp_op Some (case_sum buf2 buf2')
-       (comp_op (\<lambda>_. None) (\<lambda>_. []) (aeq_op (case_sum (BTL pb buf1) (BTL pb buf1')))
-         (id_op buf1''))
-       (aeq_op (case_sum buf3 buf3')))\<close>
-          using that by fastforce
-        thus ?thesis by (fastforce intro: bc_sym[OF bc_base])
-      qed
-      moreover have "\<exists>op2'. step Tau (map_op projl projr (comp_op Some (case_sum buf2 buf2') (comp_op (\<lambda>_. None) (\<lambda>_. []) (aeq_op (case_sum buf1 buf1')) (id_op buf1'')) (aeq_op (case_sum buf3 buf3')))) op2' \<and> bisim_cong (\<lambda>s t. \<exists>buf1 buf1' buf1'' buf2 buf2' buf3 buf3'. s = map_op projl projr (comp_op Some (case_sum buf2 buf2') (comp_op (\<lambda>_. None) (\<lambda>_. []) (aeq_op (case_sum buf1 buf1')) (id_op buf1'')) (aeq_op (case_sum buf3 buf3'))) \<and> t = map_op (case_sum Inr Inl) id (map_op projl projr (comp_op Some (case_sum buf2' buf2) (comp_op (\<lambda>_. None) (\<lambda>_. []) (id_op buf1'') (aeq_op (case_sum buf1 buf1'))) (aeq_op (case_sum buf3' buf3))))) (map_op (case_sum Inr Inl) id (map_op projl projr (comp_op Some (case_sum buf2' buf2) (comp_op (\<lambda>_. None) (\<lambda>_. []) (id_op buf1'') (aeq_op (case_sum buf1 buf1'))) (aeq_op (case_sum (BTL pa buf3') (BTL pa buf3)))))) op2'"
-        if "buf3' pa \<noteq> []"
-          and "buf3 pa \<noteq> []"
-          and "BHD pa buf3' \<noteq> BHD pa buf3"
-          and "pa \<notin> defaults"
-        for pa :: 'a
-        using that by (intro exI conjI[rotated, OF bc_sym[OF bc_base]], auto)
-      ultimately show ?thesis
-        using H by (auto elim !: step_map_op_elim step_comp_op_elim step_aeq_op_elim step_id_op_cases)
-    qed
+    apply -
+    explore (auto elim!: step_comp_op_elim step_map_op_elim step_aeq_op_elim step_id_op_cases split: if_splits sum.splits; hypsubst_thin)
+  proof -
+    have "\<exists>op2'. wstep (Inp (Inl (Inl pb)) y) (map_op assoc id (map_op projl projr (comp_op Some (case_sum B2'' B2) (comp_op (\<lambda>_. None) (\<lambda>_. []) (id_op B1'') (aeq_op (case_sum B1' B1))) (aeq_op (case_sum B3'' B3))))) op2' \<and> \<W> (\<lambda>op1xx op2xx. \<exists>A A1 A1' B1' A2 A3 A1'' A2' A3'. op1xx = map_op projl projr (comp_op Some (case_sum A2' A2) (comp_op (\<lambda>_. None) (\<lambda>_. []) (aeq_op (case_sum A1'' A1')) (id_op A1)) (aeq_op (case_sum A3' A3))) \<and> (\<exists>B1 B2 B3 B1'' B2'' B3''. op2xx = map_op assoc id (map_op projl projr (comp_op Some (case_sum B2'' B2) (comp_op (\<lambda>_. None) (\<lambda>_. []) (id_op B1'') (aeq_op (case_sum B1' B1))) (aeq_op (case_sum B3'' B3)))) \<and> A = (A1 >> A2) >> A3 \<and> (\<forall>p. \<exists>m n. A1'' p = drop n (((B1'' >> B2'') >> B3'') p) \<and> (\<exists>C'. A1' p = drop n (C' p) \<and> B1' p = drop m (C' p) \<and> B1 p = drop m (A p) \<and> (A2' >> A3') p = tested n (C' p) (((B1'' >> B2'') >> B3'') p) \<and> (B2 >> B3) p = tested m (A p) (C' p) \<and> n \<le> length (C' p) \<and> n \<le> length (((B1'' >> B2'') >> B3'') p) \<and> m \<le> length (C' p) \<and> m \<le> length (A p))))) (map_op projl projr (comp_op Some (case_sum A2' A2) (comp_op (\<lambda>_. None) (\<lambda>_. []) (aeq_op (case_sum (BENQ pb y A1'') A1')) (id_op A1)) (aeq_op (case_sum A3' A3)))) op2'"
+      if "\<forall>p. \<exists>m n. A1'' p = drop n (((B1'' >> B2'') >> B3'') p) \<and> (\<exists>C'. A1' p = drop n (C' p) \<and> B1' p = drop m (C' p) \<and> B1 p = drop m (((A1 >> A2) >> A3) p) \<and> (A2' >> A3') p = tested n (C' p) (((B1'' >> B2'') >> B3'') p) \<and> (B2 >> B3) p = tested m (((A1 >> A2) >> A3) p) (C' p) \<and> n \<le> length (C' p) \<and> n \<le> length (((B1'' >> B2'') >> B3'') p) \<and> m \<le> length (C' p) \<and> m \<le> length (((A1 >> A2) >> A3) p))"
+        and "pb \<notin> defaults"
+      for pb :: 'a
+        and y :: 'b
+      using that sorry
+    moreover have "\<exists>op2'. wstep (Inp (Inl (Inr pb)) y) (map_op assoc id (map_op projl projr (comp_op Some (case_sum B2'' B2) (comp_op (\<lambda>_. None) (\<lambda>_. []) (id_op B1'') (aeq_op (case_sum B1' B1))) (aeq_op (case_sum B3'' B3))))) op2' \<and> \<W> (\<lambda>op1xx op2xx. \<exists>A A1 A1' B1' A2 A3 A1'' A2' A3'. op1xx = map_op projl projr (comp_op Some (case_sum A2' A2) (comp_op (\<lambda>_. None) (\<lambda>_. []) (aeq_op (case_sum A1'' A1')) (id_op A1)) (aeq_op (case_sum A3' A3))) \<and> (\<exists>B1 B2 B3 B1'' B2'' B3''. op2xx = map_op assoc id (map_op projl projr (comp_op Some (case_sum B2'' B2) (comp_op (\<lambda>_. None) (\<lambda>_. []) (id_op B1'') (aeq_op (case_sum B1' B1))) (aeq_op (case_sum B3'' B3)))) \<and> A = (A1 >> A2) >> A3 \<and> (\<forall>p. \<exists>m n. A1'' p = drop n (((B1'' >> B2'') >> B3'') p) \<and> (\<exists>C'. A1' p = drop n (C' p) \<and> B1' p = drop m (C' p) \<and> B1 p = drop m (A p) \<and> (A2' >> A3') p = tested n (C' p) (((B1'' >> B2'') >> B3'') p) \<and> (B2 >> B3) p = tested m (A p) (C' p) \<and> n \<le> length (C' p) \<and> n \<le> length (((B1'' >> B2'') >> B3'') p) \<and> m \<le> length (C' p) \<and> m \<le> length (A p))))) (map_op projl projr (comp_op Some (case_sum A2' A2) (comp_op (\<lambda>_. None) (\<lambda>_. []) (aeq_op (case_sum A1'' (BENQ pb y A1'))) (id_op A1)) (aeq_op (case_sum A3' A3)))) op2'"
+      if "\<forall>p. \<exists>m n. A1'' p = drop n (((B1'' >> B2'') >> B3'') p) \<and> (\<exists>C'. A1' p = drop n (C' p) \<and> B1' p = drop m (C' p) \<and> B1 p = drop m (((A1 >> A2) >> A3) p) \<and> (A2' >> A3') p = tested n (C' p) (((B1'' >> B2'') >> B3'') p) \<and> (B2 >> B3) p = tested m (((A1 >> A2) >> A3) p) (C' p) \<and> n \<le> length (C' p) \<and> n \<le> length (((B1'' >> B2'') >> B3'') p) \<and> m \<le> length (C' p) \<and> m \<le> length (((A1 >> A2) >> A3) p))"
+        and "pb \<notin> defaults"
+      for pb :: 'a
+        and y :: 'b
+      using that sorry
+    moreover have "\<exists>op2'. wstep (Inp (Inr pb) xb) (map_op assoc id (map_op projl projr (comp_op Some (case_sum B2'' B2) (comp_op (\<lambda>_. None) (\<lambda>_. []) (id_op B1'') (aeq_op (case_sum B1' B1))) (aeq_op (case_sum B3'' B3))))) op2' \<and> \<W> (\<lambda>op1xx op2xx. \<exists>A A1 A1' B1' A2 A3 A1'' A2' A3'. op1xx = map_op projl projr (comp_op Some (case_sum A2' A2) (comp_op (\<lambda>_. None) (\<lambda>_. []) (aeq_op (case_sum A1'' A1')) (id_op A1)) (aeq_op (case_sum A3' A3))) \<and> (\<exists>B1 B2 B3 B1'' B2'' B3''. op2xx = map_op assoc id (map_op projl projr (comp_op Some (case_sum B2'' B2) (comp_op (\<lambda>_. None) (\<lambda>_. []) (id_op B1'') (aeq_op (case_sum B1' B1))) (aeq_op (case_sum B3'' B3)))) \<and> A = (A1 >> A2) >> A3 \<and> (\<forall>p. \<exists>m n. A1'' p = drop n (((B1'' >> B2'') >> B3'') p) \<and> (\<exists>C'. A1' p = drop n (C' p) \<and> B1' p = drop m (C' p) \<and> B1 p = drop m (A p) \<and> (A2' >> A3') p = tested n (C' p) (((B1'' >> B2'') >> B3'') p) \<and> (B2 >> B3) p = tested m (A p) (C' p) \<and> n \<le> length (C' p) \<and> n \<le> length (((B1'' >> B2'') >> B3'') p) \<and> m \<le> length (C' p) \<and> m \<le> length (A p))))) (map_op projl projr (comp_op Some (case_sum A2' A2) (comp_op (\<lambda>_. None) (\<lambda>_. []) (aeq_op (case_sum A1'' A1')) (id_op (BENQ pb xb A1))) (aeq_op (case_sum A3' A3)))) op2'"
+      if "\<forall>p. \<exists>m n. A1'' p = drop n (((B1'' >> B2'') >> B3'') p) \<and> (\<exists>C'. A1' p = drop n (C' p) \<and> B1' p = drop m (C' p) \<and> B1 p = drop m (((A1 >> A2) >> A3) p) \<and> (A2' >> A3') p = tested n (C' p) (((B1'' >> B2'') >> B3'') p) \<and> (B2 >> B3) p = tested m (((A1 >> A2) >> A3) p) (C' p) \<and> n \<le> length (C' p) \<and> n \<le> length (((B1'' >> B2'') >> B3'') p) \<and> m \<le> length (C' p) \<and> m \<le> length (((A1 >> A2) >> A3) p))"
+        and "pb \<notin> defaults"
+      for pb :: 'a
+        and xb :: 'b
+      using that sorry
+    moreover have "\<exists>op2'. wstep (Out pa (BHD pa A3)) (map_op assoc id (map_op projl projr (comp_op Some (case_sum B2'' B2) (comp_op (\<lambda>_. None) (\<lambda>_. []) (id_op B1'') (aeq_op (case_sum B1' B1))) (aeq_op (case_sum B3'' B3))))) op2' \<and> \<W> (\<lambda>op1xx op2xx. \<exists>A A1 A1' B1' A2 A3 A1'' A2' A3'. op1xx = map_op projl projr (comp_op Some (case_sum A2' A2) (comp_op (\<lambda>_. None) (\<lambda>_. []) (aeq_op (case_sum A1'' A1')) (id_op A1)) (aeq_op (case_sum A3' A3))) \<and> (\<exists>B1 B2 B3 B1'' B2'' B3''. op2xx = map_op assoc id (map_op projl projr (comp_op Some (case_sum B2'' B2) (comp_op (\<lambda>_. None) (\<lambda>_. []) (id_op B1'') (aeq_op (case_sum B1' B1))) (aeq_op (case_sum B3'' B3)))) \<and> A = (A1 >> A2) >> A3 \<and> (\<forall>p. \<exists>m n. A1'' p = drop n (((B1'' >> B2'') >> B3'') p) \<and> (\<exists>C'. A1' p = drop n (C' p) \<and> B1' p = drop m (C' p) \<and> B1 p = drop m (A p) \<and> (A2' >> A3') p = tested n (C' p) (((B1'' >> B2'') >> B3'') p) \<and> (B2 >> B3) p = tested m (A p) (C' p) \<and> n \<le> length (C' p) \<and> n \<le> length (((B1'' >> B2'') >> B3'') p) \<and> m \<le> length (C' p) \<and> m \<le> length (A p))))) (map_op projl projr (comp_op Some (case_sum A2' A2) (comp_op (\<lambda>_. None) (\<lambda>_. []) (aeq_op (case_sum A1'' A1')) (id_op A1)) (aeq_op (case_sum (BTL pa A3') (BTL pa A3))))) op2'"
+      if "\<forall>p. \<exists>m n. A1'' p = drop n (((B1'' >> B2'') >> B3'') p) \<and> (\<exists>C'. A1' p = drop n (C' p) \<and> B1' p = drop m (C' p) \<and> B1 p = drop m (((A1 >> A2) >> A3) p) \<and> (A2' >> A3') p = tested n (C' p) (((B1'' >> B2'') >> B3'') p) \<and> (B2 >> B3) p = tested m (((A1 >> A2) >> A3) p) (C' p) \<and> n \<le> length (C' p) \<and> n \<le> length (((B1'' >> B2'') >> B3'') p) \<and> m \<le> length (C' p) \<and> m \<le> length (((A1 >> A2) >> A3) p))"
+        and "A3' pa \<noteq> []"
+        and "A3 pa \<noteq> []"
+        and "BHD pa A3' = BHD pa A3"
+        and "pa \<notin> defaults"
+      for pa :: 'a
+      using that 
+  apply -
+      apply (drule spec[of _ pa])
+      apply (elim conjE exE)
+      subgoal for m n C'
+        using finds_tested_first_equal[where n=n and xs="C' pa" and ys="((B1'' >> B2'') >> B3'') pa" and z="BHD pa A3'" and zs="tl ((A2' >> A3') pa)"] apply -
+        apply (drule meta_mp)
+        apply (metis BHD_BULK_BENQ_cases BHD_def BULK_BENQ_empty list.collapse)
+        apply (drule meta_mp)
+        apply assumption
+        apply (drule meta_mp)
+         apply assumption
+        apply (elim exE conjE)
+        subgoal for k
+        apply (intro exI conjI)
+         apply (rule wstep_trans(1))
+        apply (rule rtranclp_trans)
+          apply (rule progress_buffers[unfolded pcomp_op_def])
+           apply assumption
+           apply (rule refl)+
+          apply (rule test_n[unfolded pcomp_op_def, where n=k and p=pa])
+          subgoal
+            apply (subst (1 2) fun_upd_apply)
+            apply (simp (no_asm)  add: BULK_BENQ_bulk_benq)
+            apply (subst tested_min_helper[symmetric])
+               apply assumption+
+            using tested_comm apply (metis BULK_BENQ_def)
+            apply (simp add: )
+
+        find_theorems BULK_BENQ "_ @ _"
+
+
+
+
+end
+    moreover have "\<exists>op2'. (step Tau)\<^sup>*\<^sup>* (map_op assoc id (map_op projl projr (comp_op Some (case_sum B2'' B2) (comp_op (\<lambda>_. None) (\<lambda>_. []) (id_op B1'') (aeq_op (case_sum B1' B1))) (aeq_op (case_sum B3'' B3))))) op2' \<and> \<W> (\<lambda>op1xx op2xx. \<exists>A A1 A1' B1' A2 A3 A1'' A2' A3'. op1xx = map_op projl projr (comp_op Some (case_sum A2' A2) (comp_op (\<lambda>_. None) (\<lambda>_. []) (aeq_op (case_sum A1'' A1')) (id_op A1)) (aeq_op (case_sum A3' A3))) \<and> (\<exists>B1 B2 B3 B1'' B2'' B3''. op2xx = map_op assoc id (map_op projl projr (comp_op Some (case_sum B2'' B2) (comp_op (\<lambda>_. None) (\<lambda>_. []) (id_op B1'') (aeq_op (case_sum B1' B1))) (aeq_op (case_sum B3'' B3)))) \<and> A = (A1 >> A2) >> A3 \<and> (\<forall>p. \<exists>m n. A1'' p = drop n (((B1'' >> B2'') >> B3'') p) \<and> (\<exists>C'. A1' p = drop n (C' p) \<and> B1' p = drop m (C' p) \<and> B1 p = drop m (A p) \<and> (A2' >> A3') p = tested n (C' p) (((B1'' >> B2'') >> B3'') p) \<and> (B2 >> B3) p = tested m (A p) (C' p) \<and> n \<le> length (C' p) \<and> n \<le> length (((B1'' >> B2'') >> B3'') p) \<and> m \<le> length (C' p) \<and> m \<le> length (A p))))) (map_op projl projr (comp_op Some (case_sum A2' (BENQ pb (BHD pb A1) A2)) (comp_op (\<lambda>_. None) (\<lambda>_. []) (aeq_op (case_sum A1'' A1')) (id_op (BTL pb A1))) (aeq_op (case_sum A3' A3)))) op2'"
+      if "\<forall>p. \<exists>m n. A1'' p = drop n (((B1'' >> B2'') >> B3'') p) \<and> (\<exists>C'. A1' p = drop n (C' p) \<and> B1' p = drop m (C' p) \<and> B1 p = drop m (((A1 >> A2) >> A3) p) \<and> (A2' >> A3') p = tested n (C' p) (((B1'' >> B2'') >> B3'') p) \<and> (B2 >> B3) p = tested m (((A1 >> A2) >> A3) p) (C' p) \<and> n \<le> length (C' p) \<and> n \<le> length (((B1'' >> B2'') >> B3'') p) \<and> m \<le> length (C' p) \<and> m \<le> length (((A1 >> A2) >> A3) p))"
+        and "pb \<notin> defaults"
+        and "A1 pb \<noteq> []"
+      for pb :: 'a
+      using that sorry
+    moreover have "\<exists>op2'. (step Tau)\<^sup>*\<^sup>* (map_op assoc id (map_op projl projr (comp_op Some (case_sum B2'' B2) (comp_op (\<lambda>_. None) (\<lambda>_. []) (id_op B1'') (aeq_op (case_sum B1' B1))) (aeq_op (case_sum B3'' B3))))) op2' \<and> \<W> (\<lambda>op1xx op2xx. \<exists>A A1 A1' B1' A2 A3 A1'' A2' A3'. op1xx = map_op projl projr (comp_op Some (case_sum A2' A2) (comp_op (\<lambda>_. None) (\<lambda>_. []) (aeq_op (case_sum A1'' A1')) (id_op A1)) (aeq_op (case_sum A3' A3))) \<and> (\<exists>B1 B2 B3 B1'' B2'' B3''. op2xx = map_op assoc id (map_op projl projr (comp_op Some (case_sum B2'' B2) (comp_op (\<lambda>_. None) (\<lambda>_. []) (id_op B1'') (aeq_op (case_sum B1' B1))) (aeq_op (case_sum B3'' B3)))) \<and> A = (A1 >> A2) >> A3 \<and> (\<forall>p. \<exists>m n. A1'' p = drop n (((B1'' >> B2'') >> B3'') p) \<and> (\<exists>C'. A1' p = drop n (C' p) \<and> B1' p = drop m (C' p) \<and> B1 p = drop m (A p) \<and> (A2' >> A3') p = tested n (C' p) (((B1'' >> B2'') >> B3'') p) \<and> (B2 >> B3) p = tested m (A p) (C' p) \<and> n \<le> length (C' p) \<and> n \<le> length (((B1'' >> B2'') >> B3'') p) \<and> m \<le> length (C' p) \<and> m \<le> length (A p))))) (map_op projl projr (comp_op Some (case_sum (BENQ pb (BHD pb A1') A2') A2) (comp_op (\<lambda>_. None) (\<lambda>_. []) (aeq_op (case_sum (BTL pb A1'') (BTL pb A1'))) (id_op A1)) (aeq_op (case_sum A3' A3)))) op2'"
+      if "\<forall>p. \<exists>m n. A1'' p = drop n (((B1'' >> B2'') >> B3'') p) \<and> (\<exists>C'. A1' p = drop n (C' p) \<and> B1' p = drop m (C' p) \<and> B1 p = drop m (((A1 >> A2) >> A3) p) \<and> (A2' >> A3') p = tested n (C' p) (((B1'' >> B2'') >> B3'') p) \<and> (B2 >> B3) p = tested m (((A1 >> A2) >> A3) p) (C' p) \<and> n \<le> length (C' p) \<and> n \<le> length (((B1'' >> B2'') >> B3'') p) \<and> m \<le> length (C' p) \<and> m \<le> length (((A1 >> A2) >> A3) p))"
+        and "A1'' pb \<noteq> []"
+        and "A1' pb \<noteq> []"
+        and "BHD pb A1'' = BHD pb A1'"
+        and "pb \<notin> defaults"
+      for pb :: 'a
+      using that sorry
+    moreover have "\<exists>op2'. (step Tau)\<^sup>*\<^sup>* (map_op assoc id (map_op projl projr (comp_op Some (case_sum B2'' B2) (comp_op (\<lambda>_. None) (\<lambda>_. []) (id_op B1'') (aeq_op (case_sum B1' B1))) (aeq_op (case_sum B3'' B3))))) op2' \<and> \<W> (\<lambda>op1xx op2xx. \<exists>A A1 A1' B1' A2 A3 A1'' A2' A3'. op1xx = map_op projl projr (comp_op Some (case_sum A2' A2) (comp_op (\<lambda>_. None) (\<lambda>_. []) (aeq_op (case_sum A1'' A1')) (id_op A1)) (aeq_op (case_sum A3' A3))) \<and> (\<exists>B1 B2 B3 B1'' B2'' B3''. op2xx = map_op assoc id (map_op projl projr (comp_op Some (case_sum B2'' B2) (comp_op (\<lambda>_. None) (\<lambda>_. []) (id_op B1'') (aeq_op (case_sum B1' B1))) (aeq_op (case_sum B3'' B3)))) \<and> A = (A1 >> A2) >> A3 \<and> (\<forall>p. \<exists>m n. A1'' p = drop n (((B1'' >> B2'') >> B3'') p) \<and> (\<exists>C'. A1' p = drop n (C' p) \<and> B1' p = drop m (C' p) \<and> B1 p = drop m (A p) \<and> (A2' >> A3') p = tested n (C' p) (((B1'' >> B2'') >> B3'') p) \<and> (B2 >> B3) p = tested m (A p) (C' p) \<and> n \<le> length (C' p) \<and> n \<le> length (((B1'' >> B2'') >> B3'') p) \<and> m \<le> length (C' p) \<and> m \<le> length (A p))))) (map_op projl projr (comp_op Some (case_sum (BTL pa A2') A2) (comp_op (\<lambda>_. None) (\<lambda>_. []) (aeq_op (case_sum A1'' A1')) (id_op A1)) (aeq_op (case_sum (BENQ pa (BHD pa A2') A3') A3)))) op2'"
+      if "\<forall>p. \<exists>m n. A1'' p = drop n (((B1'' >> B2'') >> B3'') p) \<and> (\<exists>C'. A1' p = drop n (C' p) \<and> B1' p = drop m (C' p) \<and> B1 p = drop m (((A1 >> A2) >> A3) p) \<and> (A2' >> A3') p = tested n (C' p) (((B1'' >> B2'') >> B3'') p) \<and> (B2 >> B3) p = tested m (((A1 >> A2) >> A3) p) (C' p) \<and> n \<le> length (C' p) \<and> n \<le> length (((B1'' >> B2'') >> B3'') p) \<and> m \<le> length (C' p) \<and> m \<le> length (((A1 >> A2) >> A3) p))"
+        and "A2' pa \<noteq> []"
+        and "pa \<notin> defaults"
+      for pa :: 'a
+      using that sorry
+    moreover have "\<exists>op2'. (step Tau)\<^sup>*\<^sup>* (map_op assoc id (map_op projl projr (comp_op Some (case_sum B2'' B2) (comp_op (\<lambda>_. None) (\<lambda>_. []) (id_op B1'') (aeq_op (case_sum B1' B1))) (aeq_op (case_sum B3'' B3))))) op2' \<and> \<W> (\<lambda>op1xx op2xx. \<exists>A A1 A1' B1' A2 A3 A1'' A2' A3'. op1xx = map_op projl projr (comp_op Some (case_sum A2' A2) (comp_op (\<lambda>_. None) (\<lambda>_. []) (aeq_op (case_sum A1'' A1')) (id_op A1)) (aeq_op (case_sum A3' A3))) \<and> (\<exists>B1 B2 B3 B1'' B2'' B3''. op2xx = map_op assoc id (map_op projl projr (comp_op Some (case_sum B2'' B2) (comp_op (\<lambda>_. None) (\<lambda>_. []) (id_op B1'') (aeq_op (case_sum B1' B1))) (aeq_op (case_sum B3'' B3)))) \<and> A = (A1 >> A2) >> A3 \<and> (\<forall>p. \<exists>m n. A1'' p = drop n (((B1'' >> B2'') >> B3'') p) \<and> (\<exists>C'. A1' p = drop n (C' p) \<and> B1' p = drop m (C' p) \<and> B1 p = drop m (A p) \<and> (A2' >> A3') p = tested n (C' p) (((B1'' >> B2'') >> B3'') p) \<and> (B2 >> B3) p = tested m (A p) (C' p) \<and> n \<le> length (C' p) \<and> n \<le> length (((B1'' >> B2'') >> B3'') p) \<and> m \<le> length (C' p) \<and> m \<le> length (A p))))) (map_op projl projr (comp_op Some (case_sum A2' (BTL pa A2)) (comp_op (\<lambda>_. None) (\<lambda>_. []) (aeq_op (case_sum A1'' A1')) (id_op A1)) (aeq_op (case_sum A3' (BENQ pa (BHD pa A2) A3))))) op2'"
+      if "\<forall>p. \<exists>m n. A1'' p = drop n (((B1'' >> B2'') >> B3'') p) \<and> (\<exists>C'. A1' p = drop n (C' p) \<and> B1' p = drop m (C' p) \<and> B1 p = drop m (((A1 >> A2) >> A3) p) \<and> (A2' >> A3') p = tested n (C' p) (((B1'' >> B2'') >> B3'') p) \<and> (B2 >> B3) p = tested m (((A1 >> A2) >> A3) p) (C' p) \<and> n \<le> length (C' p) \<and> n \<le> length (((B1'' >> B2'') >> B3'') p) \<and> m \<le> length (C' p) \<and> m \<le> length (((A1 >> A2) >> A3) p))"
+        and "A2 pa \<noteq> []"
+        and "pa \<notin> defaults"
+      for pa :: 'a
+      using that sorry
+    moreover have "\<exists>op2'. (step Tau)\<^sup>*\<^sup>* (map_op assoc id (map_op projl projr (comp_op Some (case_sum B2'' B2) (comp_op (\<lambda>_. None) (\<lambda>_. []) (id_op B1'') (aeq_op (case_sum B1' B1))) (aeq_op (case_sum B3'' B3))))) op2' \<and> \<W> (\<lambda>op1xx op2xx. \<exists>A A1 A1' B1' A2 A3 A1'' A2' A3'. op1xx = map_op projl projr (comp_op Some (case_sum A2' A2) (comp_op (\<lambda>_. None) (\<lambda>_. []) (aeq_op (case_sum A1'' A1')) (id_op A1)) (aeq_op (case_sum A3' A3))) \<and> (\<exists>B1 B2 B3 B1'' B2'' B3''. op2xx = map_op assoc id (map_op projl projr (comp_op Some (case_sum B2'' B2) (comp_op (\<lambda>_. None) (\<lambda>_. []) (id_op B1'') (aeq_op (case_sum B1' B1))) (aeq_op (case_sum B3'' B3)))) \<and> A = (A1 >> A2) >> A3 \<and> (\<forall>p. \<exists>m n. A1'' p = drop n (((B1'' >> B2'') >> B3'') p) \<and> (\<exists>C'. A1' p = drop n (C' p) \<and> B1' p = drop m (C' p) \<and> B1 p = drop m (A p) \<and> (A2' >> A3') p = tested n (C' p) (((B1'' >> B2'') >> B3'') p) \<and> (B2 >> B3) p = tested m (A p) (C' p) \<and> n \<le> length (C' p) \<and> n \<le> length (((B1'' >> B2'') >> B3'') p) \<and> m \<le> length (C' p) \<and> m \<le> length (A p))))) (map_op projl projr (comp_op Some (case_sum A2' A2) (comp_op (\<lambda>_. None) (\<lambda>_. []) (aeq_op (case_sum (BTL pb A1'') (BTL pb A1'))) (id_op A1)) (aeq_op (case_sum A3' A3)))) op2'"
+      if "\<forall>p. \<exists>m n. A1'' p = drop n (((B1'' >> B2'') >> B3'') p) \<and> (\<exists>C'. A1' p = drop n (C' p) \<and> B1' p = drop m (C' p) \<and> B1 p = drop m (((A1 >> A2) >> A3) p) \<and> (A2' >> A3') p = tested n (C' p) (((B1'' >> B2'') >> B3'') p) \<and> (B2 >> B3) p = tested m (((A1 >> A2) >> A3) p) (C' p) \<and> n \<le> length (C' p) \<and> n \<le> length (((B1'' >> B2'') >> B3'') p) \<and> m \<le> length (C' p) \<and> m \<le> length (((A1 >> A2) >> A3) p))"
+        and "A1'' pb \<noteq> []"
+        and "A1' pb \<noteq> []"
+        and "BHD pb A1'' \<noteq> BHD pb A1'"
+        and "pb \<notin> defaults"
+      for pb :: 'a
+ using that 
+      apply -
+      apply (drule spec[of _ pb])
+      apply (elim conjE exE)
+      subgoal for m n C'
+        apply (intro exI conjI)
+         apply fast
+        apply (rule wbcr_base)
+        apply (intro exI conjI)
+           apply (rule refl)+
+        apply (intro allI)
+        subgoal for p
+          apply (cases "p = pb")
+          subgoal
+            apply hypsubst_thin
+            apply (rule exI[of _ m])
+            apply (rule exI[of _ "Suc n"])
+            apply (intro conjI)
+            subgoal
+              by (metis BTL_access drop_Suc tl_drop)
+            subgoal
+            apply (rule exI[of _ C'])
+              apply (intro conjI)
+              apply simp_all
+               apply (metis BTL_access drop_Suc tl_drop)
+              apply (rule tested_diff_Suc_gen[symmetric])
+              using nat_less_le apply blast
+              using nless_le apply blast
+              apply (metis BHD_def hd_drop_conv_nth nat_less_le)
+              done
+            done
+          subgoal
+            using that(1) apply -
+            apply (drule spec[of _ p])
+      apply (elim conjE exE)
+            subgoal for m' n' C''
+            apply (rule exI[of _ m'])
+              apply (rule exI[of _ "n'"])
+              apply simp
+              apply (intro conjI)
+              subgoal
+                by (metis BTL_diff_access)
+              apply (rule exI[of _ C''])
+              apply (intro conjI)
+              apply simp_all
+              apply (metis BTL_diff_access)
+              done
+            done
+          done
+        done
+      done
+    moreover have "\<exists>op2'. (step Tau)\<^sup>*\<^sup>* (map_op assoc id (map_op projl projr (comp_op Some (case_sum B2'' B2) (comp_op (\<lambda>_. None) (\<lambda>_. []) (id_op B1'') (aeq_op (case_sum B1' B1))) (aeq_op (case_sum B3'' B3))))) op2' \<and> \<W> (\<lambda>op1xx op2xx. \<exists>A A1 A1' B1' A2 A3 A1'' A2' A3'. op1xx = map_op projl projr (comp_op Some (case_sum A2' A2) (comp_op (\<lambda>_. None) (\<lambda>_. []) (aeq_op (case_sum A1'' A1')) (id_op A1)) (aeq_op (case_sum A3' A3))) \<and> (\<exists>B1 B2 B3 B1'' B2'' B3''. op2xx = map_op assoc id (map_op projl projr (comp_op Some (case_sum B2'' B2) (comp_op (\<lambda>_. None) (\<lambda>_. []) (id_op B1'') (aeq_op (case_sum B1' B1))) (aeq_op (case_sum B3'' B3)))) \<and> A = (A1 >> A2) >> A3 \<and> (\<forall>p. \<exists>m n. A1'' p = drop n (((B1'' >> B2'') >> B3'') p) \<and> (\<exists>C'. A1' p = drop n (C' p) \<and> B1' p = drop m (C' p) \<and> B1 p = drop m (A p) \<and> (A2' >> A3') p = tested n (C' p) (((B1'' >> B2'') >> B3'') p) \<and> (B2 >> B3) p = tested m (A p) (C' p) \<and> n \<le> length (C' p) \<and> n \<le> length (((B1'' >> B2'') >> B3'') p) \<and> m \<le> length (C' p) \<and> m \<le> length (A p))))) (map_op projl projr (comp_op Some (case_sum A2' A2) (comp_op (\<lambda>_. None) (\<lambda>_. []) (aeq_op (case_sum A1'' A1')) (id_op A1)) (aeq_op (case_sum (BTL pa A3') (BTL pa A3))))) op2'"
+      if "\<forall>p. \<exists>m n. A1'' p = drop n (((B1'' >> B2'') >> B3'') p) \<and> (\<exists>C'. A1' p = drop n (C' p) \<and> B1' p = drop m (C' p) \<and> B1 p = drop m (((A1 >> A2) >> A3) p) \<and> (A2' >> A3') p = tested n (C' p) (((B1'' >> B2'') >> B3'') p) \<and> (B2 >> B3) p = tested m (((A1 >> A2) >> A3) p) (C' p) \<and> n \<le> length (C' p) \<and> n \<le> length (((B1'' >> B2'') >> B3'') p) \<and> m \<le> length (C' p) \<and> m \<le> length (((A1 >> A2) >> A3) p))"
+        and "A3' pa \<noteq> []"
+        and "A3 pa \<noteq> []"
+        and "BHD pa A3' \<noteq> BHD pa A3"
+        and "pa \<notin> defaults"
+      for pa :: 'a
+      using that sorry
+    ultimately show ?thesis
+      using SIM1  by (auto elim !: step_comp_op_elim step_map_op_elim step_aeq_op_elim step_id_op_cases split: if_splits sum.splits)
   qed
+
+
+
+end
+next
+  case SIM2
+  then show ?case sorry
 qed
 
+
+end
+
 lemma A1:
-  \<open>(\<Q> \<parallel> \<I>) \<bullet> \<Q> ~ map_op (case_sum Inr Inl) id ((\<I> \<parallel> \<Q>) \<bullet> \<Q>)\<close>
+  \<open>(\<Q> \<parallel> \<I>) \<bullet> \<Q> ~ map_op assoc id ((\<I> \<parallel> \<Q>) \<bullet> \<Q>)\<close>
   unfolding scomp_op_def
   using A1_gen[of \<open>\<lambda>_. []\<close> \<open>\<lambda>_. []\<close> \<open>\<lambda>_. []\<close> \<open>\<lambda>_. []\<close> \<open>\<lambda>_. []\<close> \<open>\<lambda>_. []\<close> \<open>\<lambda>_. []\<close>]
   by simp
